Veritas.Verifier.CorrectDefs.fst
@@ -213,3 +213,4 @@ let rec lemma_thread_id (il:t_verifiable_log):
   if n = 0 then ()
   else
     lemma_thread_id (id, hprefix l)
+
